backend/Lineartyping.v
@@ -106,7 +106,7 @@ Inductive wt_instr : instruction -> Prop :=
   | wt_Ljumptable:
       forall arg tbl,
       mreg_type arg = Tint ->
-      list_length_z tbl * 4 <= Int.max_signed ->
+      list_length_z tbl * 4 <= Int.max_unsigned ->
       wt_instr (Ljumptable arg tbl)
   | wt_Lreturn: 
       wt_instr (Lreturn).
