backend/RTLtyping.v
@@ -123,7 +123,7 @@ Inductive wt_instr : instruction -> Prop :=
       forall arg tbl,
       env arg = Tint ->
       (forall s, In s tbl -> valid_successor s) ->
-      list_length_z tbl * 4 <= Int.max_signed ->
+      list_length_z tbl * 4 <= Int.max_unsigned ->
       wt_instr (Ijumptable arg tbl)
   | wt_Ireturn: 
       forall optres,
@@ -245,7 +245,7 @@ Definition check_instr (i: instruction) : bool :=
   | Ijumptable arg tbl =>
       check_reg arg Tint
       && List.forallb check_successor tbl
-      && zle (list_length_z tbl * 4) Int.max_signed
+      && zle (list_length_z tbl * 4) Int.max_unsigned
   | Ireturn optres =>
       match optres, funct.(fn_sig).(sig_res) with
       | None, None => true
